cp

src/tls/ConnInvariant.fst
@@ -37,6 +37,12 @@ let registered (i:id{StAE.is_stream_ae i}) (w:StreamAE.writer i) (c:connection) 
       (let i' = Handshake.hsId (Handshake.Epoch.h e) in
         i=i' /\ StAE.stream_ae #i e.w == w))
 
+let writer_separated_from_all_handshakes (#i:AE.id) (w:AE.writer i) (conn:c_tab) = 
+  forall n.{:pattern (MM.sel conn n)}
+       match MM.sel conn n with 
+       | Some c -> HH.disjoint (HS.region (C.hs c)) (StreamAE.State.region w) 
+       | None -> True
+
 let ms_conn_inv (ms:ms_tab)
  		(conn:c_tab)
 		(h:HyperHeap.t) 
@@ -45,18 +51,24 @@ let ms_conn_inv (ms:ms_tab)
      (match MM.sel ms i with 
       | None -> True
       | Some w -> 
-	Map.contains h (StreamAE.State.region w) /\ //technical for framing; need to know that the writer's region exists
+	//technical: for framing; need to know that the writer's region exists
+	Map.contains h (StreamAE.State.region w) /\  
+	//separation: each writer is separated from every connection's handshake state, and from tls_tables_region
 	HH.disjoint (StreamAE.State.region w) tls_tables_region /\
-	(MR.m_sel h (StreamAE.ilog (StreamAE.State.log w)) = Seq.createEmpty  \/   //the writer is still unused; or
+	writer_separated_from_all_handshakes w conn /\
+	//main application invariant:
+	(MR.m_sel h (StreamAE.ilog (StreamAE.State.log w)) = Seq.createEmpty  \/   //the writer is either still unused; or
 	             (let copt = MM.sel conn (I.nonce_of_id i) in
-  		      is_Some copt /\ registered i w (Some.v copt) h)))      //it's been assigned to a connection
+  		      is_Some copt /\ registered i w (Some.v copt) h)))            //it's been registered with the connection associated with its nonce
 
 let ms_conn_invariant (ms:ms_tab)
  		      (conn:c_tab)
 		      (h:HyperHeap.t) 
   = forall (i:id) .{:pattern (MM.sel ms i)} ms_conn_inv ms conn h i
 
-let mc_inv (h:HyperHeap.t) = ms_conn_invariant (MR.m_sel h MS.ms_tab) (MR.m_sel h conn_table) h
+let mc_inv (h:HyperHeap.t) = 
+    HH.as_ref (MR.as_rref conn_table) =!= HH.as_ref (MR.as_rref MS.ms_tab)
+    /\ ms_conn_invariant (MR.m_sel h MS.ms_tab) (MR.m_sel h conn_table) h
 
 //Checking the stability of the invariant
 
@@ -64,20 +76,24 @@ let mc_inv (h:HyperHeap.t) = ms_conn_invariant (MR.m_sel h MS.ms_tab) (MR.m_sel 
 //   Easy: because a new log is empty and both cases of the conn table allow empty logs to be in ms
 val ms_derive_is_ok: h0:HyperHeap.t -> h1:HyperHeap.t -> i:AE.id -> w:MS.writer i 
   -> Lemma (requires 
+	        (let conn = MR.m_sel h0 conn_table in
+	         let old_ms = MR.m_sel h0 MS.ms_tab in 
+		 let new_ms = MR.m_sel h1 MS.ms_tab in
 		 HH.contains_ref (MR.as_rref conn_table) h0 /\
-		 HH.contains_ref (MR.as_rref MS.ms_tab) h0 /\
-		 Map.contains h1 (StreamAE.State.region w) /\
-		 HH.disjoint (StreamAE.State.region w) tls_tables_region /\
+		 HH.contains_ref (MR.as_rref MS.ms_tab) h0  /\
+		 Map.contains h1 (StreamAE.State.region w)  /\
 		 mc_inv h0 /\ //we're initially in the invariant
+		 HH.disjoint (StreamAE.State.region w) tls_tables_region /\
+		 writer_separated_from_all_handshakes w conn /\
 		 HH.modifies (Set.singleton tls_tables_region) h0 h1 /\ //we just changed the tls_region
 		 HH.modifies_rref tls_tables_region !{HH.as_ref (MR.as_rref MS.ms_tab)} h0 h1 /\ //and within it, at most the ms_tab
-		 (let old_ms = MR.m_sel h0 MS.ms_tab in 
-		  let new_ms = MR.m_sel h1 MS.ms_tab in
- 		  old_ms = new_ms //either ms_tab didn't change at all
+		 (old_ms = new_ms //either ms_tab didn't change at all
 		  \/ (MM.sel old_ms i = None /\
 		     new_ms = MM.upd old_ms i w /\ //or we just added w to it
-	   	     (TLSInfo.authId i ==> MR.m_sel h1 (AE.ilog (StreamAE.State.log w)) = Seq.createEmpty)))) //and it is a fresh log
+	   	     (TLSInfo.authId i ==> MR.m_sel h1 (AE.ilog (StreamAE.State.log w)) = Seq.createEmpty))))) //and it is a fresh log
 	 (ensures (mc_inv h1))
+(* assume val gadmit: f:(unit -> GTot Type0) -> Tot (u:unit{f()}) *)
+
 let ms_derive_is_ok h0 h1 i w = 
   let aux :  j:id -> Lemma (let new_ms = MR.m_sel h1 MS.ms_tab in
 			  let new_conn = MR.m_sel h1 conn_table in
@@ -85,8 +101,10 @@ let ms_derive_is_ok h0 h1 i w =
     fun j -> 			    
       let old_ms = MR.m_sel h0 MS.ms_tab in 
       let new_ms = MR.m_sel h1 MS.ms_tab in
+      (* let old_conn = MR.m_sel h0 conn_table in *)
       let new_conn = MR.m_sel h1 conn_table in
       assert (ms_conn_inv new_ms new_conn h1 i);
+      (* assert (old_conn = new_conn); *)
       if (authId j && StAE.is_stream_ae j)
       then match MM.sel new_ms j with 
            | None -> ()
@@ -116,66 +134,91 @@ let try_ms_derive (r:HH.rid) (i:AE.id)
     let h1 = ST.get () in 
     ms_derive_is_ok h0 h1 i w;
     w
-    
 
-(* //2. Adding a new epoch to a connection c, with a fresh index (hdId i) for c *)
-(* //      -- we found a writer w at (ms i), pre-allocated (we're second) or not (we're first) *)
-(* //      -- we need to show that the (exists e. SeqProperties.mem ...) is false (because of the fresh index for c) *)
-(* //      -- so, we're in the "not yet used" case ... so, the epoch's writer is in its initial state and we can return it (our goal is to return a fresh epoch) *)
+let all_epoch_writers_share_conn_nonce (c:connection) (i:AE.id) (wi:AE.writer i) (h:HH.t)
+    : Lemma (requires (registered i wi c h))
+            (ensures (I.nonce_of_id i = c.hs.nonce))
+    = ()
 
-(* val add_epoch_ok: h0:HyperHeap.t -> h1:HyperHeap.t -> i:AE.id{authId i} *)
-(* 		-> c:r_conn (idNonce i) -> e:epoch (HS.region c.hs) (HS.peer c.hs) *)
-(*   -> Lemma (requires *)
-(*             (let ctab = MR.m_sel h0 conn_table in *)
-(* 	     let mstab = MR.m_sel h0 MS.ms_tab in *)
-(* 	     let old_hs_log = HH.sel h0 (HS.log c.hs) in *)
-(*      	     let new_hs_log = HH.sel h1 (HS.log c.hs) in *)
-(* 	     let rgn = HS.region c.hs in *)
-(* 	     HH.contains_ref (MR.as_rref conn_table) h0 /\ *)
-(* 	     HH.contains_ref (MR.as_rref MS.ms_tab) h0 /\ *)
-(* 	     HH.disjoint (HS.region c.hs) tls_region /\ *)
-(* 	     HH.contains_ref (HS.log c.hs) h0 /\ *)
-(* 	     HH.contains_ref (HS.log c.hs) h1 /\ *)
-(* 	     mc_inv h0 /\ //we're initially in the invariant *)
-(* 	     i=hsId (Epoch.h e) /\ //the epoch has id it *)
-(* 	     (let w = StAE.stream_ae #i (Epoch.w e) in //the epoch writer *)
-(* 	      let epochs = HH.sel h0 (HS.log c.hs) in *)
-(*       	      Map.contains h1 (StreamAE.State.region w) /\ *)
-(* 	      (forall e. SeqProperties.mem e epochs ==> hsId (Epoch.h e) <> i) /\ //i is fresh for c *)
-(*  	      MM.sel mstab (i, rgn) = Some w /\ //we found the writer in the ms_tab *)
-(* 	      MM.sel ctab (idNonce i) = Some c /\ //we found the connection in the conn_table *)
-(* 	      HH.modifies_one (HS.region c.hs) h0 h1 /\ //we just modified this connection's handshake region *)
-(* 	      HH.modifies_rref (HS.region c.hs) !{HH.as_ref (HS.log c.hs)} h0 h1 /\ //and within it, just the epochs log *)
-(* 	      new_hs_log = SeqProperties.snoc old_hs_log e))) //and we modified it by adding this epoch to it *)
-(* 	  (ensures mc_inv h1) //we're back in the invariant *)
+#reset-options "--z3timeout 10 --initial_ifuel 2 --initial_fuel 0"
 
-(* #reset-options "--z3timeout 10 --initial_fuel 2 --max_fuel 2 --initial_ifuel 2 --max_ifuel 2" *)
+let writer_registered_to_at_most_one_connection 
+    (n1:random) (c1:r_conn n1)
+    (n2:random) (c2:r_conn n2{n1 <> n2})
+    (i:AE.id {I.nonce_of_id i = n1}) (w:AE.writer i) (h:HH.t)
+    : Lemma (requires (registered i w c1 h))
+	    (ensures (~ (registered i w c2 h)))
+    = ()
 
-(* let add_epoch_ok h0 h1 i c e =  *)
-(*   assert (MR.m_sel h0 MS.ms_tab = MR.m_sel h1 MS.ms_tab); *)
-(*   assert (MR.m_sel h0 conn_table = MR.m_sel h1 conn_table); *)
-(*   let w = StAE.stream_ae #i (Epoch.w e) in //the epoch writer *)
-(*   assert (MR.m_sel h0 (StreamAE.ilog (StreamAE.State.log w)) = MR.m_sel h1 (StreamAE.ilog (StreamAE.State.log w))); *)
-(*   let ctab = MR.m_sel h0 conn_table in *)
-(*   let mstab = MR.m_sel h0 MS.ms_tab in *)
-(*   let copt = MM.sel ctab (idNonce i) in *)
-(*   let old_hs_log = HH.sel h0 (HS.log c.hs) in *)
-(*   assert (is_Some copt); *)
-(*   assert (~ (registered i w (Some.v copt) h0)); *)
-(*   MonotoneSeq.lemma_mem_snoc old_hs_log e; *)
-(*   assert (registered i w (Some.v copt) h1); *)
-(*   let j : id  = magic () in  *)
-(*   let s : HH.rid = magic () in  *)
-(*   assume (StAE.is_stream_ae j); *)
-(*   assume (authId j); *)
-(*   assume (s <> HS.region c.hs); *)
-(*   match MM.sel mstab (j, s) with  *)
-(*   | None -> admit() *)
-(*   | Some wj ->  *)
-(*     assume (StreamAE.State.region wj <> HS.region c.hs); //can see here why the post-condition fails ... need better separation invariants between the HS.log and the writer logs *)
-(*     assume (HH.contains_ref (MR.as_rref (StreamAE.ilog (StreamAE.State.log wj))) h0); *)
-(*     assert (MR.m_sel h0 (StreamAE.ilog (StreamAE.State.log wj)) = MR.m_sel h1 (StreamAE.ilog (StreamAE.State.log wj))); *)
-(*     admit() *)
+let writer_region_within_connection
+    (n:random) (c:r_conn n)
+    (i:AE.id {I.nonce_of_id i = n}) (w:AE.writer i) (h:HH.t)
+    : Lemma (requires (registered i w c h))
+	    (ensures (HH.includes (C.region c) (StreamAE.State.region w)))
+    = ()
+
+#reset-options "--z3timeout 10 --initial_fuel 2 --max_fuel 2 --initial_ifuel 2 --max_ifuel 2"
+
+//2. Adding a new epoch to a connection c, with a fresh index (hdId i) for c
+//      -- we found a writer w at (ms i), pre-allocated (we're second) or not (we're first)
+//      -- we need to show that the (exists e. SeqProperties.mem ...) is false (because of the fresh index for c)
+//      -- so, we're in the "not yet used" case ... so, the epoch's writer is in its initial state and we can return it (our goal is to return a fresh epoch)
+val register_writer_in_epoch_ok: h0:HyperHeap.t -> h1:HyperHeap.t -> i:AE.id{authId i}
+		-> c:r_conn (I.nonce_of_id i) -> e:epoch (HS.region c.hs) (I.nonce_of_id i)
+  -> Lemma (requires
+            (let ctab = MR.m_sel h0 conn_table in
+	     let mstab = MR.m_sel h0 MS.ms_tab in
+	     let old_hs_log = HH.sel h0 (HS.log c.hs) in
+     	     let new_hs_log = HH.sel h1 (HS.log c.hs) in
+	     let rgn = HS.region c.hs in
+	     HH.contains_ref (MR.as_rref conn_table) h0 /\
+	     HH.contains_ref (MR.as_rref MS.ms_tab) h0 /\
+	     HH.disjoint (HS.region c.hs) tls_region /\
+	     HH.contains_ref (HS.log c.hs) h0 /\
+	     HH.contains_ref (HS.log c.hs) h1 /\
+	     mc_inv h0 /\ //we're initially in the invariant
+	     i=hsId (Epoch.h e) /\ //the epoch has id i
+	     (let w = StAE.stream_ae #i (Epoch.w e) in //the epoch writer
+	      let epochs = HH.sel h0 (HS.log c.hs) in
+              N.registered (I.nonce_of_id i) (HH.parent (StreamAE.State.region w)) /\ 
+	      HH.disjoint (HH.parent (StreamAE.State.region w)) tls_region /\
+      	      Map.contains h1 (StreamAE.State.region w) /\
+	      (forall e. SeqProperties.mem e epochs ==> hsId (Epoch.h e) <> i) /\ //i is fresh for c
+ 	      MM.sel mstab i = Some w /\ //we found the writer in the ms_tab
+	      MM.sel ctab (I.nonce_of_id i) = Some c /\ //we found the connection in the conn_table
+	      HH.modifies_one (HS.region c.hs) h0 h1 /\ //we just modified this connection's handshake region
+	      HH.modifies_rref (HS.region c.hs) !{HH.as_ref (HS.log c.hs)} h0 h1 /\ //and within it, just the epochs log
+	      new_hs_log = SeqProperties.snoc old_hs_log e))) //and we modified it by adding this epoch to it
+	  (ensures mc_inv h1) //we're back in the invariant
+
+
+#reset-options "--z3timeout 10 --initial_ifuel 2 --initial_fuel 0"
+
+let register_writer_in_epoch_ok h0 h1 i c e = 
+  assert (MR.m_sel h0 MS.ms_tab = MR.m_sel h1 MS.ms_tab);
+  assert (MR.m_sel h0 conn_table = MR.m_sel h1 conn_table);
+  let w = StAE.stream_ae #i (Epoch.w e) in //the epoch writer
+  assert (MR.m_sel h0 (StreamAE.ilog (StreamAE.State.log w)) = MR.m_sel h1 (StreamAE.ilog (StreamAE.State.log w)));
+  let ctab = MR.m_sel h0 conn_table in
+  let mstab = MR.m_sel h0 MS.ms_tab in
+  let copt = MM.sel ctab (I.nonce_of_id i) in
+  let old_hs_log = HH.sel h0 (HS.log c.hs) in
+  assert (is_Some copt);
+  assert (~ (registered i w (Some.v copt) h0));
+  MonotoneSeq.lemma_mem_snoc old_hs_log e;
+  assert (registered i w (Some.v copt) h1);
+  let j : id  = magic () in
+  let nonce = I.nonce_of_id i in 
+  assume (StAE.is_stream_ae j);
+  assume (authId j);
+  match MM.sel mstab j with
+  | None -> admit()
+  | Some wj ->
+    assume (registered j wj c h0);
+    assert (HH.disjoint (StreamAE.State.region wj) (HS.region c.hs)); //can see here why the post-condition fails ... need better separation invariants between the HS.log and the writer logs
+    assume (HH.contains_ref (MR.as_rref (StreamAE.ilog (StreamAE.State.log wj))) h0);
+    assert (MR.m_sel h0 (StreamAE.ilog (StreamAE.State.log wj)) = MR.m_sel h1 (StreamAE.ilog (StreamAE.State.log wj)));
+    admit()
 
 
 //3. Adding to a log registered in a connection: Need to prove that ms_conn_invariant is maintained
